theories/computational.v
@@ -1,0 +1,93 @@
+Require Import refframe.base.
+Require Import stdpp.strings.
+Require Import stdpp.propset.
+Require Import refframe.module.
+
+Import version7.
+
+Class IoPartition EV IN OUT := {
+  io_input : EV → IN;
+  io_output : EV → OUT;
+}.
+
+Record computational_module EV IN OUT `{!IoPartition EV IN OUT} := {
+  cm_state : Type;
+  cm_initial : cm_state;
+  cm_next : cm_state → IN → option (option (OUT * cm_state));
+}.
+Arguments cm_state {_ _ _ _}.
+Arguments cm_initial {_ _ _ _}.
+Arguments cm_next {_ _ _ _}.
+Definition cm_to_module {EV IN OUT} `{!IoPartition EV IN OUT} (cm : computational_module EV IN OUT) : module EV := {|
+  m_state := option cm.(cm_state);
+  m_initial := Some cm.(cm_initial);
+  m_step σ e σ' := if σ is Some σm then if e is Some κ then
+                     match cm.(cm_next) σm (io_input κ) with
+                     | None => False
+                     | Some None => σ' = None
+                     | Some (Some (out, σm')) => σ' = Some σm' ∧ io_output κ = out
+                     end
+                   else False else False;
+  m_is_ub σ := σ = None;
+|}.
+Coercion cm_to_module : computational_module >-> module.
+
+Module test.
+Inductive call_event : Type :=
+| CRecvCallEvt (fn : string) (args: list Z) | CRecvRetEvt (ret: Z)
+| CCallEvt (fn : string) (args: list Z) | CDoneEvt (ret: Z).
+
+Inductive call_event_in : Type :=
+| InRecvCallEvt (fn : string) (args: list Z) | InRecvRetEvt (ret: Z)
+| InCallEvt | InDoneEvt.
+Inductive call_event_out : Type :=
+| OutRecvCallEvt | OutRecvRetEvt
+| OutCallEvt (fn : string) (args: list Z) | OutDoneEvt (ret: Z).
+Global Instance call_event_partition : IoPartition call_event call_event_in call_event_out := {|
+  io_input e := match e with
+                | CRecvCallEvt fn args => InRecvCallEvt fn args
+                | CRecvRetEvt ret => InRecvRetEvt ret
+                | CCallEvt fn args => InCallEvt
+                | CDoneEvt ret => InDoneEvt
+                end;
+  io_output e := match e with
+                | CRecvCallEvt fn args => OutRecvCallEvt
+                | CRecvRetEvt ret => OutRecvRetEvt
+                | CCallEvt fn args => OutCallEvt fn args
+                | CDoneEvt ret => OutDoneEvt ret
+                end;
+|}.
+
+Inductive test_cm_state : Type :=
+| TCMInit | TCMRecvd (n : Z) | TCMWait (n : Z) | TCMRet (n : Z).
+Definition test_cm : (computational_module call_event call_event_in call_event_out)  := {|
+  cm_state := test_cm_state;
+  cm_initial := TCMInit;
+  cm_next σ i :=
+    match σ, i with
+    | TCMInit, InRecvCallEvt "test" [n] =>
+      Some (Some (OutRecvCallEvt, TCMRecvd n))
+    | TCMRecvd n, InCallEvt =>
+      Some (Some (OutCallEvt "id" [n], TCMWait n))
+    | TCMWait n, InRecvRetEvt ret =>
+      if bool_decide (n = ret) then
+        Some (Some (OutRecvRetEvt, TCMRet n))
+      else Some None
+    | TCMRet n, InDoneEvt =>
+      Some (Some (OutDoneEvt n, TCMInit))
+    | _, _ => None
+    end
+  ;
+|}.
+
+Goal ∀ n, ∃ σ,
+      has_trace test_cm (Some TCMInit) [Vis (CRecvCallEvt "test" [n]); Vis (CCallEvt "id" [n]); Vis (CRecvRetEvt n); Vis (CDoneEvt n)] σ.
+Proof.
+  move => ?. eexists _.
+  apply: TraceStepSome. done.
+  apply: TraceStepSome. done.
+  apply: TraceStepSome. simpl. case_bool_decide => //.
+  apply: TraceStepSome. done.
+  apply: TraceEnd.
+Qed.
+End test.
